crypto/bignum/x25519/Hacl.Spec.EC.AddAndDouble2.fst
@@ -8,38 +8,64 @@ open Hacl.Spec.Bignum.Fmul
 open Hacl.Spec.EC.AddAndDouble
 
 
-#set-options "--initial_fuel 0 --max_fuel 0"
+#set-options "--initial_fuel 0 --max_fuel 0 --z3rlimit 10"
+
+let s_513 = s:seqelem{red_513 s}
+
+let lemma_53_is_5413 (s:seqelem{red_53 s}) : Lemma (red_5413 s) = ()
+let lemma_513_is_53 (s:seqelem{red_513 s}) : Lemma (red_53 s) = ()
+let lemma_513_is_55 (s:seqelem{red_513 s}) : Lemma (red_55 s) = ()
+let lemma_513_is_5413 (s:seqelem{red_513 s}) : Lemma (red_5413 s) = ()
+let lemma_513_is_52 (s:seqelem{red_513 s}) : Lemma (red_52 s) = ()
 
 val fmonty_tot:
-  px:seqelem{red_52 px} -> pz:seqelem{red_52 pz} ->
-  pqx:seqelem{red_52 pqx} -> pqz:seqelem{red_52 pqz} ->
-  qx:seqelem{red_52 qx} ->
-  Tot (seqelem * seqelem * seqelem * seqelem)
+  px:s_513 -> pz:s_513 ->
+  pqx:s_513 -> pqz:s_513 ->
+  qx:s_513 ->
+  Tot (s_513 * s_513 * s_513 * s_513)
 let fmonty_tot px pz pqx pqz qx =
-  fsum_52_is_53 px pz;
+  fsum_513_is_53 px pz;
   let px' = fsum_tot px pz in
-  lemma_fdifference_unrolled' pz px;
+  lemma_fdifference_unrolled'' pz px;
+  lemma_fdifference_unrolled''' pz px;
   let pz' = fdifference_tot pz px in
-  fsum_52_is_53 pqx pqz;
+  fsum_513_is_53 pqx pqz;
   let pqx' = fsum_tot pqx pqz in
-  lemma_fdifference_unrolled' pqz pqx;
+  lemma_fdifference_unrolled'' pqz pqx;
   let pqz' = fdifference_tot pqz pqx in
   fmul_53_55_is_fine pqx' pz';
   let xxprime = fmul_tot pqx' pz' in
   fmul_53_55_is_fine px' pqz';
   let zzprime = fmul_tot px' pqz' in
-  fsum_52_is_53 xxprime zzprime;
+  fsum_513_is_53 xxprime zzprime;
   let xxprime' = fsum_tot xxprime zzprime in
-  lemma_fdifference_unrolled' zzprime pqx;
+  lemma_fdifference_unrolled''' zzprime pqx;
   let zzprime' = fdifference_tot zzprime pqx in
+  lemma_53_is_5413 xxprime';
+  fsquare_5413_is_fine xxprime';
   let x3 = fsquare_times_tot xxprime' 1 in
+  fsquare_5413_is_fine zzprime';
   let zzzprime = fsquare_times_tot zzprime' 1 in
+  lemma_513_is_53 zzzprime; lemma_513_is_55 qx;
+  fmul_53_55_is_fine zzzprime qx;
   let z3 = fmul_tot zzzprime qx in
+  lemma_53_is_5413 px';
+  fsquare_5413_is_fine px';
   let xx = fsquare_times_tot px' 1 in
+  fsquare_5413_is_fine pz';
   let zz = fsquare_times_tot pz' 1 in
+  lemma_513_is_53 xx;
+  lemma_513_is_55 zz;
+  fmul_53_55_is_fine xx zz;
   let x2 = fmul_tot xx zz in
+  lemma_fdifference_unrolled'' zz xx;  
   let zz' = fdifference_tot zz xx in
+  let scalar = (uint64_to_limb Hacl.Bignum.Constants.a24) in
+  fscalar_is_fine zz scalar;
   let zzz = fscalar_tot zz (uint64_to_limb Hacl.Bignum.Constants.a24) in
+  lemma_513_is_52 xx;
+  fsum_52_is_53 zzz xx;
   let zzz' = fsum_tot zzz xx in
-  let z2 = fsum_tot zz' zzz' in
+  fmul_53_55_is_fine zzz' zz';
+  let z2 = fmul_tot zzz' zz' in
   (x2, z2, x3, z3)
